<!--
author:   U. Anthony Omegbu
email:    anthonyomegbu@gmail.com
version:  0.0.1

tags:     LiaScript, education, OER

logo:     https://your-logo-url.com/logo.jpg

comment:  This document is a simple LiaScript course example.

-->

# Algebra 2 

Algebra II Spring Final 2023 FINAL REVIEW Solution Guide
========================================================

Unit 8: EXPONENTS AND RADICALS
------------------------------

 Simplify the expressions using exponent rules.

1. b4⋅b3b^4 \\cdot b^3b4⋅b3
   
   **Solution:** When multiplying expressions with the same base, we add the exponents. So, b4⋅b3\=b4+3\=b7b^4 \\cdot b^3 = b^{4+3} = b^7b4⋅b3\=b4+3\=b7.

2. c5⋅c2⋅c2c^5\\cdot c^2 \\cdot c^2c5⋅c2⋅c2
   
   **Solution:** Similarly, for this expression, we add all the exponents: c5⋅c2⋅c2\=c5+2+2\=c9c^5\\cdot c^2 \\cdot c^2 = c^{5+2+2} = c^9c5⋅c2⋅c2\=c5+2+2\=c9.

3. a−4⋅a−3a^{-4} \\cdot a^{-3}a−4⋅a−3
   
   **Solution:** The rule of adding exponents applies here as well. Negative exponents indicate that the base is on the denominator of a fraction. However, for this problem, we just add the exponents: a−4⋅a−3\=a−4−3\=a−7a^{-4} \\cdot a^{-3} = a^{-4-3} = a^{-7}a−4⋅a−3\=a−4−3\=a−7.

4. x5⋅x−4⋅xx^5 \\cdot x^{-4} \\cdot xx5⋅x−4⋅x
   
   **Solution:** In this case, we add the exponents, and remember that xxx is the same as x1x^1x1. So, x5⋅x−4⋅x\=x5+(−4)+1\=x2x^5 \\cdot x^{-4} \\cdot x = x^{5+(-4)+1} = x^2x5⋅x−4⋅x\=x5+(−4)+1\=x2.

5. (2x)2(4y)2(2x)^2(4y)^2(2x)2(4y)2
   
   **Solution:** When raising a power to a power, we multiply the exponents. Also, remember that both the coefficient and the variable are raised to the power. So, (2x)2(4y)2\=(22x2)(42y2)\=4x2⋅16y2\=64x2y2(2x)^2(4y)^2 = (2^2x^2)(4^2y^2) = 4x^2 \\cdot 16y^2 = 64x^2y^2(2x)2(4y)2\=(22x2)(42y2)\=4x2⋅16y2\=64x2y2.

6. −2gh(g3h5)\-2gh(g^3h^5)−2gh(g3h5)
   
   **Solution:** In this case, we multiply the like terms. So, −2gh(g3h5)\=−2g1h1⋅g3h5\=−2g1+3h1+5\=−2g4h6\-2gh(g^3h^5) = -2g^1h^1 \\cdot g^3h^5 = -2g^{1+3}h^{1+5} = -2g^4h^6−2gh(g3h5)\=−2g1h1⋅g3h5\=−2g1+3h1+5\=−2g4h6.

7. 10x2y3(10xy8)10x^2y^3(10xy^8)10x2y3(10xy8)
   
   **Solution:** Here, we multiply the coefficients and add the exponents of like terms. So, 10x2y3(10xy8)\=10⋅10⋅x2+1y3+8\=100x3y1110x^2y^3(10xy^8) = 10 \\cdot 10 \\cdot x^{2+1}y^{3+8} = 100x^3y^{11}10x2y3(10xy8)\=10⋅10⋅x2+1y3+8\=100x3y11.

8. 24wz23w3z5\\frac{24wz^2}{3w^3z^5}3w3z524wz2​
   
   **Solution:** For this expression, we simplify the coefficients by division and subtract the exponents of like terms (numerator - denominator). So, 24wz23w3z5\=243⋅w1−3z2−5\=8w−2z−3\\frac{24wz^2}{3w^3z^5} = \\frac{24}{3} \\cdot w^{1-3}z^{2-5} = 8w^{-2}z^{-3}3w3z524wz2​\=324​⋅w1−3z2−5\=8w−2z−3. This can also be written as 8w2z3\\frac{8}{w^2z^3}w2z38​ if you prefer not to have negative exponents.

9. c23c^{\\frac{2}{3}}c32​

**Solution:** The expression c23c^{\\frac{2}{3}}c32​ can be rewritten in radical notation as c23\\sqrt\[3\]{c^2}3c2​. This is because the denominator of the fraction in the exponent represents the root (in this case, the cube root), and the numerator represents the power (in this case, squared).

16. x16x^{\\frac{1}{6}}x61​

**Solution:** Similarly, the expression x16x^{\\frac{1}{6}}x61​ can be rewritten in radical notation as x6\\sqrt\[6\]{x}6x​. Here, the denominator of the fraction in the exponent is 6, which represents the sixth root, and the numerator is 1, which represents the first power (or simply xxx).

17. 16x13\\sqrt{16x^{13}}16x13​

**Solution:** The square root of 16 is 4. For x13x^{13}x13, we can take out pairs of xxx's as x2x^2x2. There are 6 pairs and one xxx left inside the square root. So, 16x13\=4x6x\\sqrt{16x^{13}} = 4x^6\\sqrt{x}16x13​\=4x6x​.

18. 27a6b23\\sqrt\[3\]{27a^6b^2}327a6b2​

**Solution:** The cube root of 27 is 3. For a6a^6a6, we can take out pairs of a3a^3a3 as there are 2 pairs. For b2b^2b2, there aren't enough bbb's to take out of the cube root, so it stays inside. So, 27a6b23\=3a2b23\\sqrt\[3\]{27a^6b^2} = 3a^2\\sqrt\[3\]{b^2}327a6b2​\=3a23b2​.

19. (3c)9\\sqrt{(3c)^9}(3c)9​

**Solution:** When taking the square root of a term raised to an odd power, we can take out half of the power (rounded down) and leave the rest inside the square root. The square root of 393^939 is 343^434 (since 4.54.54.5 rounds down to 444), and the square root of c9c^9c9 is c4cc^4\\sqrt{c}c4c​. So, (3c)9\=34c43c\=81c43c\\sqrt{(3c)^9} = 3^4c^4\\sqrt{3c} = 81c^4\\sqrt{3c}(3c)9​\=34c43c​\=81c43c​.

21. 32+50−483\\sqrt{2} + \\sqrt{50} - 4\\sqrt{8}32​+50​−48​

**Solution:** We can simplify each term first. 50\\sqrt{50}50​ simplifies to 525\\sqrt{2}52​ and 8\\sqrt{8}8​ simplifies to 222\\sqrt{2}22​. Substituting these simplifications back into the original expression gives us 32+52−4∗223\\sqrt{2} + 5\\sqrt{2} - 4\*2\\sqrt{2}32​+52​−4∗22​. Combining like terms, we find that the expression simplifies to 0.

22. 4(29−5)4\\left(2\\sqrt{9} - 5\\right)4(29​−5)

**Solution:** We can simplify inside the parentheses first. 292\\sqrt{9}29​ simplifies to 2∗3\=62\*3 = 62∗3\=6. Substituting this simplification back into the original expression gives us 4(6−5)4\\left(6 - 5\\right)4(6−5), which simplifies to 4∗1\=44\*1 = 44∗1\=4.

24. (1+27)(5+7)(1 + 2\\sqrt{7})(5 + \\sqrt{7})(1+27​)(5+7​)

**Solution:** We can use the distributive property (also known as the FOIL method) to expand this expression.

First, we multiply the first terms in each binomial: 1⋅5\=51 \\cdot 5 = 51⋅5\=5.

Next, we multiply the outer terms: 1⋅7\=71 \\cdot \\sqrt{7} = \\sqrt{7}1⋅7​\=7​.

Then, we multiply the inner terms: 27⋅5\=1072\\sqrt{7} \\cdot 5 = 10\\sqrt{7}27​⋅5\=107​.

Finally, we multiply the last terms: 27⋅7\=2⋅7\=142\\sqrt{7} \\cdot \\sqrt{7} = 2 \\cdot 7 = 1427​⋅7​\=2⋅7\=14.

Adding these results together, we get 5+7+107+14\=19+1175 + \\sqrt{7} + 10\\sqrt{7} + 14 = 19 + 11\\sqrt{7}5+7​+107​+14\=19+117​.

27. Find the area of the triangle given the following characteristics: b\=10xb = 10xb\=10x, h\=4x2h = 4x^2h\=4x2, A\=12bhA = \\frac{1}{2}bhA\=21​bh

**Solution:** We can substitute the given values of bbb and hhh into the formula for the area of a triangle, which is A\=12bhA = \\frac{1}{2}bhA\=21​bh.

Substituting b\=10xb = 10xb\=10x and h\=4x2h = 4x^2h\=4x2 into the formula gives us A\=12⋅10x⋅4x2\=20x3A = \\frac{1}{2} \\cdot 10x \\cdot 4x^2 = 20x^3A\=21​⋅10x⋅4x2\=20x3.

So, the area of the triangle is 20x320x^320x3 square units.

28. −144\\sqrt{-144}−144​

**Solution:** The square root of a negative number is an imaginary number. The square root of -144 is equal to the square root of 144 times the square root of -1. The square root of 144 is 12, and the square root of -1 is denoted as iii. So, −144\=12i\\sqrt{-144} = 12i−144​\=12i.

29. 9i39i^39i3

**Solution:** The power of iii cycles every four powers: i1\=ii^1 = ii1\=i, i2\=−1i^2 = -1i2\=−1, i3\=−ii^3 = -ii3\=−i, i4\=1i^4 = 1i4\=1, i5\=ii^5 = ii5\=i, and so on. So, i3\=−ii^3 = -ii3\=−i. Therefore, 9i3\=9(−i)\=−9i9i^3 = 9(-i) = -9i9i3\=9(−i)\=−9i.

30. (6i−8)+(−3i+2)(6i - 8) + (-3i + 2)(6i−8)+(−3i+2)

**Solution:** We can combine like terms to simplify this expression. 6i−3i\=3i6i - 3i = 3i6i−3i\=3i and −8+2\=−6\-8 + 2 = -6−8+2\=−6. So, (6i−8)+(−3i+2)\=3i−6(6i - 8) + (-3i + 2) = 3i - 6(6i−8)+(−3i+2)\=3i−6, or 3(−2+i)3(-2 + i)3(−2+i) in standard form.

31. 4i(i+2)4i(i + 2)4i(i+2)

**Solution:** We can distribute 4i4i4i to both terms inside the parentheses: 4i⋅i\=4i24i \\cdot i = 4i^24i⋅i\=4i2 and 4i⋅2\=8i4i \\cdot 2 = 8i4i⋅2\=8i. Remember that i2\=−1i^2 = -1i2\=−1, so 4i2\=4(−1)\=−44i^2 = 4(-1) = -44i2\=4(−1)\=−4. Therefore, 4i(i+2)\=−4+8i4i(i + 2) = -4 + 8i4i(i+2)\=−4+8i, or 4(−1+2i)4(-1 + 2i)4(−1+2i) in standard form.

34. 123−i\\frac{12}{3-i}3−i12​

**Solution:** To simplify a complex fraction, we can multiply the numerator and the denominator by the conjugate of the denominator. The conjugate of 3−i3 - i3−i is 3+i3 + i3+i. So, we multiply the fraction by 3+i3+i\\frac{3 + i}{3 + i}3+i3+i​ to get 12(3+i)(3−i)(3+i)\\frac{12(3 + i)}{(3 - i)(3 + i)}(3−i)(3+i)12(3+i)​. The denominator simplifies to 32−(−i)2\=9−(−1)\=103^2 - (-i)^2 = 9 - (-1) = 1032−(−i)2\=9−(−1)\=10. So, the fraction simplifies to 6(3+i)5\\frac{6(3 + i)}{5}56(3+i)​, or 3.6+1.2i3.6 + 1.2i3.6+1.2i in decimal form.

35. −2⋅−9\\sqrt{-2} \\cdot \\sqrt{-9}−2​⋅−9​

**Solution:** The square root of a negative number is an imaginary number. The square root of -2 is i2i\\sqrt{2}i2​, and the square root of -9 is 3i3i3i. So, −2⋅−9\=i2⋅3i\=−32\\sqrt{-2} \\cdot \\sqrt{-9} = i\\sqrt{2} \\cdot 3i = -3\\sqrt{2}−2​⋅−9​\=i2​⋅3i\=−32​. The negative sign comes from the fact that i⋅i\=i2\=−1i \\cdot i = i^2 = -1i⋅i\=i2\=−1.

36. f(x)\=−x+3+2f(x) = -\\sqrt{x} + 3 + 2f(x)\=−x​+3+2

**Solution:**

**Transformations:**

* The negative sign in front of the square root function reflects the graph over the x-axis.
* The "+3" inside the square root function shifts the graph 3 units to the left.
* The "+2" outside the square root function shifts the graph 2 units up.

To graph this function, start with the graph of y\=xy = \\sqrt{x}y\=x​, then apply the transformations in the order listed above.

37. f(x)\=2x−1−4f(x) = 2\\sqrt{x} - 1 - 4f(x)\=2x​−1−4

**Solution:**

**Transformations:**

* The "2" in front of the square root function vertically stretches the graph by a factor of 2.
* The "-1" inside the square root function shifts the graph 1 unit to the right.
* The "-4" outside the square root function shifts the graph 4 units down.

To graph this function, start with the graph of y\=xy = \\sqrt{x}y\=x​, then apply the transformations in the order listed above.

Note: For both functions, the transformations are applied in the order of reflection, horizontal shift, and then vertical shift.

38. x+3\=5\\sqrt{x} + 3 = 5x​+3\=5

**Solution:** To solve this equation, we first isolate the square root term by subtracting 3 from both sides of the equation: x\=5−3\=2\\sqrt{x} = 5 - 3 = 2x​\=5−3\=2. Then, we square both sides to eliminate the square root: x\=22\=4x = 2^2 = 4x\=22\=4.

39. 3x−2\=73\\sqrt{x} - 2 = 73x​−2\=7

**Solution:** First, we isolate the square root term by adding 2 to both sides of the equation: 3x\=7+2\=93\\sqrt{x} = 7 + 2 = 93x​\=7+2\=9. Then, we divide both sides by 3 to get x\=93\=3\\sqrt{x} = \\frac{9}{3} = 3x​\=39​\=3. Finally, we square both sides to eliminate the square root: x\=32\=9x = 3^2 = 9x\=32\=9.

## Quizzes

Throughout the module, there will be quizzes to test your knowledge on the topics we have covered. These quizzes will help you assess your understanding and identify areas where you may need to review.

## Active Learning Strategies

During the virtual lecture, we will use active learning strategies to engage with the material and deepen our understanding. These strategies may include group discussions, problem-solving activities, and interactive simulations.

## Conclusion

By the end of this module, you should have a strong foundation in Algebra 1 and be able to apply your knowledge to solve real-world problems.

[preview-lia](https://raw.githubusercontent.com/awakwe/Algebra-2/main/README.md)

[Preview-Lia](https://liascript.github.io/course/?https://raw.githubusercontent.com/awakwe/Algebra-2/main/README.md)
